TypeChecker.v
@@ -11,21 +11,21 @@ Import ListNotations.
 Require Import AST.
 Require Import Maps.
 
-Inductive typecheck : tc_env -> t_expr -> cont_type -> Prop :=
+Inductive typecheck : t_env -> t_expr -> t_type -> Prop :=
   (* t_Num *)
   (* t_Bool *)
   (* t_Var *)
   | TC_Num: forall env n,
-    typecheck env (t_Num n) cont_Num
+    typecheck env (t_Num n) TNum
   | TC_Bool: forall env b,
-    typecheck env (t_Bool b) cont_Bool
+    typecheck env (t_Bool b) TBool
   | TC_Var: forall env x T,
     env x = Some T ->
     typecheck env (t_Var x) T
 
   (* t_If *)
   | TC_If: forall env c e1 e2 T,
-    typecheck env c cont_Bool ->
+    typecheck env c TBool ->
     typecheck env e1 T ->
     typecheck env e2 T ->
     typecheck env (t_If c e1 e2) T
@@ -33,42 +33,42 @@ Inductive typecheck : tc_env -> t_expr -> cont_type -> Prop :=
   (* t_Fun *)
   | TC_Fun: forall env x x_T e e_T,
     typecheck (update env x x_T) e e_T ->
-    typecheck env (t_Fun x x_T e) (cont_Fun x_T e_T)
+    typecheck env (t_Fun x x_T e) (TFun x_T e_T)
 
   (* t_Call *)
   | TC_Call: forall env f e e_T T,
-    typecheck env f (cont_Fun e_T T) ->
+    typecheck env f (TFun e_T T) ->
     typecheck env e e_T ->
     typecheck env (t_Call f e) T
 
   (* t_Cons *)
   | TC_Cons: forall env hd tl T,
     typecheck env hd T ->
-    typecheck env tl (cont_List T) ->
-    typecheck env (t_Cons hd tl) (cont_List T)
+    typecheck env tl (TList T) ->
+    typecheck env (t_Cons hd tl) (TList T)
 
   (* t_Nil *)
   | TC_Nil: forall env T,
-    typecheck env (t_Nil T) (cont_List T)
+    typecheck env (t_Nil T) (TList T)
 
   (* t_Binop *)
   | TC_Binop_nnn: forall env op e1 e2,
     op = op_Plus \/
     op = op_Minus ->
-    typecheck env e1 cont_Num ->
-    typecheck env e2 cont_Num ->
-    typecheck env (t_Binop op e1 e2) cont_Num
+    typecheck env e1 TNum ->
+    typecheck env e2 TNum ->
+    typecheck env (t_Binop op e1 e2) TNum
 
   | TC_Binop_nnb: forall env op e1 e2,
     op = op_Eq \/
     op = op_Neq ->
-    typecheck env e1 cont_Num ->
-    typecheck env e2 cont_Num ->
-    typecheck env (t_Binop op e1 e2) cont_Bool
+    typecheck env e1 TNum ->
+    typecheck env e2 TNum ->
+    typecheck env (t_Binop op e1 e2) TBool
 
   | TC_Binop_bbb: forall env op e1 e2,
     op = op_And \/
     op = op_Or ->
-    typecheck env e1 cont_Bool ->
-    typecheck env e2 cont_Bool ->
-    typecheck env (t_Binop op e1 e2) cont_Bool.
+    typecheck env e1 TBool ->
+    typecheck env e2 TBool ->
+    typecheck env (t_Binop op e1 e2) TBool.
