TypeInferencer.v
@@ -12,14 +12,14 @@ Require Import AST.
 Require Import Maps.
 
 
-Inductive typeinf : ti_env -> nat -> ut_expr -> (nat * inft_type * constr) % type -> Prop :=
+Inductive typeinf : t_env -> nat -> ut_expr -> (nat * t_type * constr) % type -> Prop :=
   (* ut_Num *)
   (* ut_Bool *)
   (* ut_Var *)
   | TI_Num: forall env n fv,
-    typeinf env fv (ut_Num n) (fv, inft_Num, [])
+    typeinf env fv (ut_Num n) (fv, TNum, [])
   | TI_Bool: forall env b fv,
-    typeinf env fv (ut_Bool b) (fv, inft_Bool, [])
+    typeinf env fv (ut_Bool b) (fv, TBool, [])
   | TI_Var: forall env x fv T,
     env x = Some T -> typeinf env fv (ut_Var x) (fv, T, [])
 
@@ -32,14 +32,14 @@ Inductive typeinf : ti_env -> nat -> ut_expr -> (nat * inft_type * constr) % typ
     typeinf env fv c (c_fv, c_T, c_C) ->
     typeinf env c_fv  e1 (e1_fv, e1_T, e1_C) ->
     typeinf env e1_fv  e2 (e2_fv, e2_T, e2_C) ->
-    typeinf env fv (ut_If c e1 e2) (e2_fv, e1_T, e2_C ++ e1_C ++ c_C ++ [(e1_T, e2_T); (c_T, inft_Bool)])
+    typeinf env fv (ut_If c e1 e2) (e2_fv, e1_T, e2_C ++ e1_C ++ c_C ++ [(e1_T, e2_T); (c_T, TBool)])
 
   (* ut_Fun *)
   | TI_Fun:
     forall env fv
       x e e_fv e_C e_T,
-    typeinf (update env x (inft_Var (Id fv))) (fv + 1)  e (e_fv, e_T, e_C) ->
-    typeinf env fv (ut_Fun x e) (e_fv, (inft_Fun (inft_Var (Id fv)) e_T), e_C)
+    typeinf (update env x (TVar (Id fv))) (fv + 1)  e (e_fv, e_T, e_C) ->
+    typeinf env fv (ut_Fun x e) (e_fv, (TFun (TVar (Id fv)) e_T), e_C)
 
   (* ut_Call *)
   | TI_Call:
@@ -48,7 +48,7 @@ Inductive typeinf : ti_env -> nat -> ut_expr -> (nat * inft_type * constr) % typ
       e e_fv e_C e_T,
     typeinf env fv f (f_fv, f_T, f_C) ->
     typeinf env f_fv e (e_fv, e_T, e_C) ->
-    typeinf env fv (ut_Call f e) (e_fv + 1, inft_Var (Id e_fv), e_C ++ f_C ++ [(f_T, inft_Fun e_T (inft_Var (Id e_fv)))])
+    typeinf env fv (ut_Call f e) (e_fv + 1, TVar (Id e_fv), e_C ++ f_C ++ [(f_T, TFun e_T (TVar (Id e_fv)))])
 
   (* ut_Cons *)
   | TI_Cons:
@@ -57,12 +57,12 @@ Inductive typeinf : ti_env -> nat -> ut_expr -> (nat * inft_type * constr) % typ
       tl tl_fv tl_C tl_T,
     typeinf env fv hd (hd_fv, hd_T, hd_C) ->
     typeinf env hd_fv tl (tl_fv, tl_T, tl_C) ->
-    typeinf env fv (ut_Cons hd tl) (tl_fv, inft_List hd_T, tl_C ++ hd_C ++ [(tl_T, inft_List hd_T)])
+    typeinf env fv (ut_Cons hd tl) (tl_fv, TList hd_T, tl_C ++ hd_C ++ [(tl_T, TList hd_T)])
 
   (* ut_Nil *)
   | TI_Nil:
     forall env fv,
-    typeinf env fv ut_Nil (fv + 1, inft_List (inft_Var (Id fv)), [])
+    typeinf env fv ut_Nil (fv + 1, TList (TVar (Id fv)), [])
 
   (* ut_Binop *)
   | TI_Binop_nnn:
@@ -73,7 +73,7 @@ Inductive typeinf : ti_env -> nat -> ut_expr -> (nat * inft_type * constr) % typ
     typeinf env e1_fv e2 (e2_fv, e2_T, e2_C) ->
     op = op_Plus \/
     op = op_Minus ->
-    typeinf env fv (ut_Binop op e1 e2) (e2_fv, inft_Num, e2_C++ e1_C ++ [(e2_T, inft_Num); (e1_T, inft_Num)])
+    typeinf env fv (ut_Binop op e1 e2) (e2_fv, TNum, e2_C++ e1_C ++ [(e2_T, TNum); (e1_T, TNum)])
 
   | TI_Binop_nnb:
     forall env fv op
@@ -83,7 +83,7 @@ Inductive typeinf : ti_env -> nat -> ut_expr -> (nat * inft_type * constr) % typ
     typeinf env e1_fv e2 (e2_fv, e2_T, e2_C) ->
     op = op_Eq \/
     op = op_Neq ->
-    typeinf env fv (ut_Binop op e1 e2) (e2_fv, inft_Bool, e2_C++ e1_C ++ [(e2_T, inft_Num); (e1_T, inft_Num)])
+    typeinf env fv (ut_Binop op e1 e2) (e2_fv, TBool, e2_C++ e1_C ++ [(e2_T, TNum); (e1_T, TNum)])
 
   | TI_Binop_bbb:
     forall env fv op
@@ -93,17 +93,17 @@ Inductive typeinf : ti_env -> nat -> ut_expr -> (nat * inft_type * constr) % typ
     typeinf env e1_fv e2 (e2_fv, e2_T, e2_C) ->
     op = op_And \/
     op = op_Or ->
-    typeinf env fv (ut_Binop op e1 e2) (e2_fv, inft_Bool, e2_C++ e1_C ++ [(e2_T, inft_Bool); (e1_T, inft_Bool)]).
+    typeinf env fv (ut_Binop op e1 e2) (e2_fv, TBool, e2_C++ e1_C ++ [(e2_T, TBool); (e1_T, TBool)]).
 
-Fixpoint subst (s : (id * inft_type) % type) (t : inft_type) : inft_type :=
+Fixpoint subst (s : (id * t_type) % type) (t : t_type) : t_type :=
   match t with
-    | inft_Num | inft_Bool => t
-    | inft_Fun x e => inft_Fun (subst s x) (subst s e)
-    | inft_List l => inft_List (subst s l)
-    | inft_Var x => let (i, sub) := s in if beq_id i x then sub else t
+    | TNum | TBool => t
+    | TFun x e => TFun (subst s x) (subst s e)
+    | TList l => TList (subst s l)
+    | TVar x => let (i, sub) := s in if beq_id i x then sub else t
   end.
 
-Definition app_substs (sub : substs) (tp : inft_type) : inft_type :=
+Definition app_substs (sub : substs) (tp : t_type) : t_type :=
   fold_right (fun s t => subst s t) tp sub.
 
 Inductive solution : substs -> constr -> Prop :=
